theories/L6_PCPS/Heap/closure_conversion.v
@@ -99,6 +99,10 @@ Section CC.
         make_closures B FV Γ C ->
         ~ f \in FV ->
         make_closures (Fcons f t xs e B) FV Γ C.
+
+  (* TODO delete after comp *)
+  Notation "a &: B" := (Intersection _ [set a] B) (at level 48, left associativity)
+                     : Ensembles_scope.
   
   Inductive Closure_conversion :
     Ensemble var -> (* Variables in the current scope *)
@@ -117,7 +121,7 @@ Section CC.
         project_vars Scope c Γ FVs S ys ys' C S' ->
         (* We do not care about ys'. Should never be accessed again so do not
          add them aτ the current scope *)
-        Closure_conversion (x |: Scope) c Γ FVs e e' C' ->
+        Closure_conversion (x &: occurs_free e :|: Scope) c Γ FVs e e' C' ->
         Closure_conversion Scope c Γ FVs (Econstr x t ys e)
                            (Econstr x t ys' (C' |[ e' ]|)) C
   | CC_Ecase :
@@ -135,7 +139,7 @@ Section CC.
       forall Scope c Γ FVs S S' x y y' C C' t N e e',
         Disjoint _ S (FV_cc Scope Γ) ->
         project_var Scope c Γ FVs S y y' C S' ->
-        Closure_conversion (x |: Scope) c Γ FVs e e' C' ->
+        Closure_conversion (x &: occurs_free e :|: Scope) c Γ FVs e e' C' ->
         Closure_conversion Scope c Γ FVs (Eproj x t N y e)
                            (Eproj x t N y' (C' |[ e' ]|)) C
   | CC_Efun :
@@ -172,7 +176,7 @@ Section CC.
       forall Scope c Γ FVs S S' x ys ys' C C' f e e',
         Disjoint _ S (FV_cc Scope Γ) ->
         project_vars Scope c Γ FVs S ys ys' C S' ->
-        Closure_conversion (x |: Scope) c Γ FVs e e' C' ->
+        Closure_conversion (x &: occurs_free e :|: Scope) c Γ FVs e e' C' ->
         Closure_conversion Scope c Γ FVs (Eprim x f ys e)
                            (Eprim x f ys' (C' |[ e' ]|)) C
   | CC_Ehalt :
@@ -197,7 +201,7 @@ Section CC.
              In _ S  Γ' ->
              make_closures B ((occurs_free e) \\ FromList ys) Γ' Cf -> 
              Closure_conversion_fundefs B c FVs defs defs' ->
-             Closure_conversion (FromList ys :|: (name_in_fundefs B :&: ((occurs_free e) \\ FromList ys)))
+             Closure_conversion ((FromList ys :|: name_in_fundefs B) :&: (occurs_free e))
                                 c Γ' FVs e e' C ->
              Closure_conversion_fundefs B c FVs (Fcons f t ys e defs )
                                         (Fcons f t (Γ' :: ys) (Cf |[ (C |[ e' ]|) ]|) defs')
